src/Lean/Elab/PreDefinition/Tailrec.lean
@@ -1,0 +1,90 @@
+/-
+Copyright (c) 2021 Microsoft Corporation. All rights reserved.
+Released under Apache 2.0 license as described in the file LICENSE.
+Authors: Leonardo de Moura
+-/
+prelude
+import Lean.Elab.PreDefinition.WF.PackMutual
+import Init.Tailrec
+
+namespace Lean.Elab
+open WF
+open Meta
+
+partial def solveMono (goal : MVarId) : MetaM Unit :=
+  goal.withContext do
+    let type ← goal.getType
+    let_expr Tailrec.mono _α _β _inst f := type |
+      throwError "Unexpected goal:{goal}"
+
+    if f.isLambda && !f.bindingBody!.hasLooseBVars then
+      let new_goals ← goal.applyConst ``Tailrec.mono_const
+      unless new_goals.isEmpty do
+        throwError "Left over goals"
+      return
+
+    if f.isLambda && f.bindingBody!.isApp && f.bindingBody!.appFn! == .bvar 0 then
+      let new_goals ← goal.applyConst ``Tailrec.mono_apply
+      unless new_goals.isEmpty do
+        throwError "Left over goals"
+      return
+
+    -- We could be more careful here and only split a match or ite that
+    -- is right under the lambda, and maybe use `apply_ite`-style lemmas to avoid the more
+    -- expesive splitter machinery. For now using `splitTarget` works fine.
+    if let some mvarIds ← splitTarget? goal (splitIte := true) then
+      mvarIds.forM solveMono
+      return
+
+    throwError "Recursive calls in non-tail position:{indentExpr type}"
+
+private def replaceRecApps (recFnName : Name) (fixedPrefixSize : Nat) (F : Expr) (e : Expr) : Expr :=
+  e.replace fun e =>
+    if e.isAppOfArity recFnName fixedPrefixSize then
+      some F
+    else
+      none
+
+def derecursifyTailrec (fixedPrefixSize : Nat) (preDef : PreDefinition) :
+    TermElabM PreDefinition := do
+  forallBoundedTelescope preDef.type fixedPrefixSize fun prefixArgs type => do
+    let type ← whnfForall type
+    unless type.isForall do
+      throwError "expected unary function type: {type}"
+    let some (α, β) := type.arrow?
+      | throwError "function has dependent type {type}"
+    let u ← getDecLevel α
+    let v ← getDecLevel β
+    let inst ← synthInstance (mkApp (.const ``Inhabited [v.succ]) β)
+    let value := mkApp3 (mkConst ``Lean.Tailrec.tailrec_fix [u, v]) α β inst
+
+    let F ← withoutModifyingEnv do
+      addAsAxiom preDef
+      let value ←
+        withLocalDeclD `F type fun f =>
+          withLocalDeclD `x α fun x => do
+            let val := preDef.value.beta (prefixArgs.push x)
+            let val := replaceRecApps preDef.declName prefixArgs.size f val
+            mkLambdaFVars #[f, x] val
+      eraseRecAppSyntaxExpr value
+    let value := .app value F
+
+    -- Now try to prove the monotonicity
+    let monoGoal := (← inferType value).bindingDomain!
+    let mono ← mkFreshExprSyntheticOpaqueMVar monoGoal
+    let goal := mono.mvarId!
+    let (_, goal) ← goal.intro1
+    mapError (f := (m!"Could not prove function to be tail-recursive:{indentD ·}")) do
+      solveMono goal
+    let value := .app value (← instantiateMVars mono)
+
+    let value ← mkLambdaFVars prefixArgs value
+    return { preDef with value }
+
+def tailRecursion (preDefs : Array PreDefinition) : TermElabM Unit := do
+  let (fixedPrefixSize, argsPacker, unaryPreDef) ← mkUnaryPreDef preDefs
+
+  let preDefNonRec : PreDefinition ← derecursifyTailrec fixedPrefixSize unaryPreDef
+  addPreDefsFromUnary preDefs fixedPrefixSize argsPacker preDefNonRec
+
+end Lean.Elab
