src/Lean/Elab/PreDefinition/WF/Main.lean
@@ -18,99 +18,16 @@ namespace Lean.Elab
 open WF
 open Meta
 
-private partial def addNonRecPreDefs (fixedPrefixSize : Nat) (argsPacker : ArgsPacker) (preDefs : Array PreDefinition) (preDefNonRec : PreDefinition)  : TermElabM Unit := do
-  let us := preDefNonRec.levelParams.map mkLevelParam
-  let all := preDefs.toList.map (·.declName)
-  for h : fidx in [:preDefs.size] do
-    let preDef := preDefs[fidx]
-    let value ← forallBoundedTelescope preDef.type (some fixedPrefixSize) fun xs _ => do
-      let value := mkAppN (mkConst preDefNonRec.declName us) xs
-      let value ← argsPacker.curryProj value fidx
-      mkLambdaFVars xs value
-    trace[Elab.definition.wf] "{preDef.declName} := {value}"
-    addNonRec { preDef with value } (applyAttrAfterCompilation := false) (all := all)
 
-partial def withCommonTelescope (preDefs : Array PreDefinition) (k : Array Expr → Array Expr → TermElabM α) : TermElabM α :=
-  go #[] (preDefs.map (·.value))
-where
-  go (fvars : Array Expr) (vals : Array Expr) : TermElabM α := do
-    if !(vals.all fun val => val.isLambda) then
-      k fvars vals
-    else if !(← vals.allM fun val => isDefEq val.bindingDomain! vals[0]!.bindingDomain!) then
-      k fvars vals
-    else
-      withLocalDecl vals[0]!.bindingName! vals[0]!.binderInfo vals[0]!.bindingDomain! fun x =>
-        go (fvars.push x) (vals.map fun val => val.bindingBody!.instantiate1 x)
-
-def getFixedPrefix (preDefs : Array PreDefinition) : TermElabM Nat :=
-  withCommonTelescope preDefs fun xs vals => do
-    let resultRef ← IO.mkRef xs.size
-    for val in vals do
-      if (← resultRef.get) == 0 then return 0
-      forEachExpr' val fun e => do
-        if preDefs.any fun preDef => e.isAppOf preDef.declName then
-          let args := e.getAppArgs
-          resultRef.modify (min args.size ·)
-          for arg in args, x in xs do
-            if !(← withoutProofIrrelevance <| withReducible <| isDefEq arg x) then
-              -- We continue searching if e's arguments are not a prefix of `xs`
-              return true
-          return false
-        else
-          return true
-    resultRef.get
-
-private def isOnlyOneUnaryDef (preDefs : Array PreDefinition) (fixedPrefixSize : Nat) : MetaM Bool := do
-  if preDefs.size == 1 then
-    lambdaTelescope preDefs[0]!.value fun xs _ => return xs.size == fixedPrefixSize + 1
-  else
-    return false
-
-/--
-Collect the names of the varying variables (after the fixed prefix); this also determines the
-arity for the well-founded translations, and is turned into an `ArgsPacker`.
-We use the term to determine the arity, but take the name from the type, for better names in the
-```
-fun : (n : Nat) → Nat | 0 => 0 | n+1 => fun n
-```
-idiom.
--/
-def varyingVarNames (fixedPrefixSize : Nat) (preDef : PreDefinition) : MetaM (Array Name) := do
-  -- We take the arity from the term, but the names from the types
-  let arity ← lambdaTelescope preDef.value fun xs _ => return xs.size
-  assert! fixedPrefixSize ≤ arity
-  if arity = fixedPrefixSize then
-    throwError "well-founded recursion cannot be used, '{preDef.declName}' does not take any (non-fixed) arguments"
-  forallBoundedTelescope preDef.type arity fun xs _ => do
-    assert! xs.size = arity
-    let xs : Array Expr := xs[fixedPrefixSize:]
-    xs.mapM (·.fvarId!.getUserName)
-
-def wfRecursion (preDefs : Array PreDefinition) (termArg?s : Array (Option TerminationArgument)) : TermElabM Unit := do
-  let termArgs? := termArg?s.mapM id -- Either all or none, checked by `elabTerminationByHints`
-  let preDefs ← preDefs.mapM fun preDef =>
-    return { preDef with value := (← preprocess preDef.value) }
-  let (fixedPrefixSize, argsPacker, unaryPreDef) ← withoutModifyingEnv do
-    for preDef in preDefs do
-      addAsAxiom preDef
-    let fixedPrefixSize ← getFixedPrefix preDefs
-    trace[Elab.definition.wf] "fixed prefix: {fixedPrefixSize}"
-    let varNamess ← preDefs.mapM (varyingVarNames fixedPrefixSize ·)
-    let argsPacker := { varNamess }
-    let preDefsDIte ← preDefs.mapM fun preDef => return { preDef with value := (← iteToDIte preDef.value) }
-    return (fixedPrefixSize, argsPacker, ← packMutual fixedPrefixSize argsPacker preDefsDIte)
-
-  let wf : TerminationArguments ← do
-    if let some tas := termArgs? then pure tas else
-    -- No termination_by here, so use GuessLex to infer one
-    guessLex preDefs unaryPreDef fixedPrefixSize argsPacker
-
-  let preDefNonRec ← forallBoundedTelescope unaryPreDef.type fixedPrefixSize fun prefixArgs type => do
+def derecursifyUnary (preDefs : Array PreDefinition) (fixedPrefixSize : Nat)
+    (argsPacker : ArgsPacker) (unaryPreDef : PreDefinition) (wf : TerminationArguments) :
+    TermElabM PreDefinition := do
+  forallBoundedTelescope unaryPreDef.type fixedPrefixSize fun prefixArgs type => do
     let type ← whnfForall type
     unless type.isForall do
       throwError "wfRecursion: expected unary function type: {type}"
     let packedArgType := type.bindingDomain!
-    elabWFRel preDefs unaryPreDef.declName prefixArgs argsPacker packedArgType wf fun wfRel => do
+    elabWFRel (preDefs.map (·.declName)) unaryPreDef.declName prefixArgs argsPacker packedArgType wf fun wfRel => do
       trace[Elab.definition.wf] "wfRel: {wfRel}"
       let (value, envNew) ← withoutModifyingEnv' do
         addAsAxiom unaryPreDef
@@ -118,39 +35,23 @@ def wfRecursion (preDefs : Array PreDefinition) (termArg?s : Array (Option Termi
         eraseRecAppSyntaxExpr value
       /- `mkFix` invokes `decreasing_tactic` which may add auxiliary theorems to the environment. -/
       let value ← unfoldDeclsFrom envNew value
-      let unaryPreDef := { unaryPreDef with value }
-      /-
-      We must remove `implemented_by` attributes from the auxiliary application because
-      this attribute is only relevant for code that is compiled. Moreover, the `[implemented_by <decl>]`
-      attribute would check whether the `unaryPreDef` type matches with `<decl>`'s type, and produce
-      and error. See issue #2899
-      -/
-      let unaryPreDef := unaryPreDef.filterAttrs fun attr => attr.name != `implemented_by
-      return unaryPreDef
+      return { unaryPreDef with value }
+
+def wfRecursion (preDefs : Array PreDefinition) (termArg?s : Array (Option TerminationArgument)) : TermElabM Unit := do
+  let termArgs? := termArg?s.mapM id -- Either all or none, checked by `elabTerminationByHints`
+  let preDefs ← preDefs.mapM fun preDef =>
+    return { preDef with value := (← preprocess preDef.value) }
+  let (fixedPrefixSize, argsPacker, unaryPreDef) ← mkUnaryPreDef preDefs
+  let unaryPreDef := { unaryPreDef with value := (← iteToDIte unaryPreDef.value) }
+
+  let wf : TerminationArguments ← do
+    if let some tas := termArgs? then pure tas else
+    -- No termination_by here, so use GuessLex to infer one
+    guessLex preDefs unaryPreDef fixedPrefixSize argsPacker
+
+  let preDefNonRec ← derecursifyUnary preDefs fixedPrefixSize argsPacker unaryPreDef wf
   trace[Elab.definition.wf] ">> {preDefNonRec.declName} :=\n{preDefNonRec.value}"
-  let preDefs ← preDefs.mapM fun d => eraseRecAppSyntax d
-  -- Do not complain if the user sets @[semireducible], which usually is a noop,
-  -- we recognize that below and then do not set @[irreducible]
-  withOptions (allowUnsafeReducibility.set · true) do
-    if (← isOnlyOneUnaryDef preDefs fixedPrefixSize) then
-      addNonRec preDefNonRec (applyAttrAfterCompilation := false)
-    else
-      withEnableInfoTree false do
-        addNonRec preDefNonRec (applyAttrAfterCompilation := false)
-      addNonRecPreDefs fixedPrefixSize argsPacker preDefs preDefNonRec
-  -- We create the `_unsafe_rec` before we abstract nested proofs.
-  -- Reason: the nested proofs may be referring to the _unsafe_rec.
-  addAndCompilePartialRec preDefs
-  let preDefs ← preDefs.mapM (abstractNestedProofs ·)
-  registerEqnsInfo preDefs preDefNonRec.declName fixedPrefixSize argsPacker
-  for preDef in preDefs do
-    markAsRecursive preDef.declName
-    generateEagerEqns preDef.declName
-    applyAttributesOf #[preDef] AttributeApplicationTime.afterCompilation
-    -- Unless the user asks for something else, mark the definition as irreducible
-    unless preDef.modifiers.attrs.any fun a =>
-      a.name = `reducible || a.name = `semireducible do
-      setIrreducibleAttribute preDef.declName
+  addPreDefsFromUnary preDefs fixedPrefixSize argsPacker preDefNonRec
 
 builtin_initialize registerTraceClass `Elab.definition.wf
 
