src/Lean/Elab/PreDefinition/WF/PackMutual.lean
@@ -1,11 +1,17 @@
 /-
 Copyright (c) 2021 Microsoft Corporation. All rights reserved.
 Released under Apache 2.0 license as described in the file LICENSE.
-Authors: Leonardo de Moura
+Authors: Leonardo de Moura, Joachim Breitner
 -/
 prelude
 import Lean.Meta.ArgsPacker
 import Lean.Elab.PreDefinition.Basic
+import Lean.Elab.PreDefinition.WF.Eqns
+
+/-!
+This module contains roughtl everything need to turn mutual n-ary functions into a single unary
+function, and is shared between well-founded recursion and tailrecursion
+-/
 
 namespace Lean.Elab.WF
 open Meta
@@ -77,5 +83,119 @@ def packMutual (fixedPrefix : Nat) (argsPacker : ArgsPacker) (preDefs : Array Pr
       (post := post fixedPrefix argsPacker (preDefs.map (·.declName)) packedDomain newFn)
     let value ← mkLambdaFVars ys value
     return { preDefNew with value }
+
+/--
+Collect the names of the varying variables (after the fixed prefix); this also determines the
+arity for the well-founded translations, and is turned into an `ArgsPacker`.
+We use the term to determine the arity, but take the name from the type, for better names in the
+```
+fun : (n : Nat) → Nat | 0 => 0 | n+1 => fun n
+```
+idiom.
+-/
+def varyingVarNames (fixedPrefixSize : Nat) (preDef : PreDefinition) : MetaM (Array Name) := do
+  -- We take the arity from the term, but the names from the types
+  let arity ← lambdaTelescope preDef.value fun xs _ => return xs.size
+  assert! fixedPrefixSize ≤ arity
+  if arity = fixedPrefixSize then
+    throwError "well-founded recursion cannot be used, '{preDef.declName}' does not take any (non-fixed) arguments"
+  forallBoundedTelescope preDef.type arity fun xs _ => do
+    assert! xs.size = arity
+    let xs : Array Expr := xs[fixedPrefixSize:]
+    xs.mapM (·.fvarId!.getUserName)
+
+
+partial def withCommonTelescope (preDefs : Array PreDefinition) (k : Array Expr → Array Expr → MetaM α) : MetaM α :=
+  go #[] (preDefs.map (·.value))
+where
+  go (fvars : Array Expr) (vals : Array Expr) : MetaM α := do
+    if !(vals.all fun val => val.isLambda) then
+      k fvars vals
+    else if !(← vals.allM fun val => isDefEq val.bindingDomain! vals[0]!.bindingDomain!) then
+      k fvars vals
+    else
+      withLocalDecl vals[0]!.bindingName! vals[0]!.binderInfo vals[0]!.bindingDomain! fun x =>
+        go (fvars.push x) (vals.map fun val => val.bindingBody!.instantiate1 x)
+
+def getFixedPrefix (preDefs : Array PreDefinition) : MetaM Nat :=
+  withCommonTelescope preDefs fun xs vals => do
+    let resultRef ← IO.mkRef xs.size
+    for val in vals do
+      if (← resultRef.get) == 0 then return 0
+      forEachExpr' val fun e => do
+        if preDefs.any fun preDef => e.isAppOf preDef.declName then
+          let args := e.getAppArgs
+          resultRef.modify (min args.size ·)
+          for arg in args, x in xs do
+            if !(← withoutProofIrrelevance <| withReducible <| isDefEq arg x) then
+              -- We continue searching if e's arguments are not a prefix of `xs`
+              return true
+          return false
+        else
+          return true
+    resultRef.get
+
+def mkUnaryPreDef (preDefs : Array PreDefinition) : MetaM (Nat × ArgsPacker × PreDefinition) :=
+  withoutModifyingEnv do
+    for preDef in preDefs do
+      addAsAxiom preDef
+    let fixedPrefixSize ← getFixedPrefix preDefs
+    trace[Elab.definition.wf] "fixed prefix: {fixedPrefixSize}"
+    let varNamess ← preDefs.mapM (varyingVarNames fixedPrefixSize ·)
+    let argsPacker := { varNamess }
+    return (fixedPrefixSize, argsPacker, ← packMutual fixedPrefixSize argsPacker preDefs)
+
+private partial def addNonRecPreDefs (fixedPrefixSize : Nat) (argsPacker : ArgsPacker) (preDefs : Array PreDefinition) (preDefNonRec : PreDefinition)  : TermElabM Unit := do
+  let us := preDefNonRec.levelParams.map mkLevelParam
+  let all := preDefs.toList.map (·.declName)
+  for h : fidx in [:preDefs.size] do
+    let preDef := preDefs[fidx]
+    let value ← forallBoundedTelescope preDef.type (some fixedPrefixSize) fun xs _ => do
+      let value := mkAppN (mkConst preDefNonRec.declName us) xs
+      let value ← argsPacker.curryProj value fidx
+      mkLambdaFVars xs value
+    trace[Elab.definition.wf] "{preDef.declName} := {value}"
+    addNonRec { preDef with value } (applyAttrAfterCompilation := false) (all := all)
+
+private def isOnlyOneUnaryDef (preDefs : Array PreDefinition) (fixedPrefixSize : Nat) : MetaM Bool := do
+  if preDefs.size == 1 then
+    lambdaTelescope preDefs[0]!.value fun xs _ => return xs.size == fixedPrefixSize + 1
+  else
+    return false
+
+def addPreDefsFromUnary (preDefs : Array PreDefinition) (fixedPrefixSize : Nat)
+    (argsPacker : ArgsPacker) (preDefNonRec : PreDefinition) : TermElabM Unit := do
+  /-
+  We must remove `implemented_by` attributes from the auxiliary application because
+  this attribute is only relevant for code that is compiled. Moreover, the `[implemented_by <decl>]`
+  attribute would check whether the `unaryPreDef` type matches with `<decl>`'s type, and produce
+  and error. See issue #2899
+  -/
+  let preDefNonRec := preDefNonRec.filterAttrs fun attr => attr.name != `implemented_by
+
+  let preDefs ← preDefs.mapM fun d => eraseRecAppSyntax d
+  -- Do not complain if the user sets @[semireducible], which usually is a noop,
+  -- we recognize that below and then do not set @[irreducible]
+  withOptions (allowUnsafeReducibility.set · true) do
+    if (← isOnlyOneUnaryDef preDefs fixedPrefixSize) then
+      addNonRec preDefNonRec (applyAttrAfterCompilation := false)
+    else
+      withEnableInfoTree false do
+        addNonRec preDefNonRec (applyAttrAfterCompilation := false)
+      addNonRecPreDefs fixedPrefixSize argsPacker preDefs preDefNonRec
+  -- We create the `_unsafe_rec` before we abstract nested proofs.
+  -- Reason: the nested proofs may be referring to the _unsafe_rec.
+  addAndCompilePartialRec preDefs
+  let preDefs ← preDefs.mapM (abstractNestedProofs ·)
+  registerEqnsInfo preDefs preDefNonRec.declName fixedPrefixSize argsPacker
+  for preDef in preDefs do
+    markAsRecursive preDef.declName
+    generateEagerEqns preDef.declName
+    applyAttributesOf #[preDef] AttributeApplicationTime.afterCompilation
+    -- Unless the user asks for something else, mark the definition as irreducible
+    unless preDef.modifiers.attrs.any fun a =>
+      a.name = `reducible || a.name = `semireducible do
+      setIrreducibleAttribute preDef.declName
+
 
 end Lean.Elab.WF
