tests/lean/run/tailrec.lean
@@ -1,0 +1,19 @@
+def find (P : Nat → Bool) (x : Nat) : Option Nat :=
+  if P x then
+    some x
+  else
+    find P (x +1)
+termination_by tailrecursion
+
+#print equations find
+
+
+/--
+error: failed to synthesize
+  Inhabited (Fin n)
+Additional diagnostic information may be available using the `set_option diagnostics true` command.
+-/
+#guard_msgs in
+def notinhabited (n m : Nat) : Fin n :=
+  notinhabited n (m+1)
+termination_by tailrecursion
